coq/audit.sh
@@ -175,6 +175,10 @@ Print Assumptions StpS.execn_exec.
 Print Assumptions StpS.exec_execn.
 Print Assumptions StpS.comp_cost.
 Print Assumptions StpS.compilation_is_step_exact.
+Print Assumptions StpS.mstepn_det.
+Print Assumptions StpS.mrunn_det_halt.
+Print Assumptions StpS.crun_cost_complete.
+Print Assumptions StpS.compilation_is_step_exact_iff.
 Print Assumptions StpS.csize_invert.
 Print Assumptions StpS.execn_rev.
 Print Assumptions StpS.execn_iff.
